@prefix owl:   <http://www.w3.org/2002/07/owl#> .
@prefix rdf:   <http://www.w3.org/1999/02/22-rdf-syntax-ns#> .
@prefix xsd:   <http://www.w3.org/2001/XMLSchema#> .
@prefix rdfs:  <http://www.w3.org/2000/01/rdf-schema#> .
@prefix fcsmps: <http://example.org/fcsmps#> .
@prefix fc:    <http://example.org/fictionalchars#> .

rdf:rest  a                 rdf:Property , rdfs:Resource ;
        rdfs:domain         rdf:List ;
        rdfs:range          rdf:List ;
        rdfs:subPropertyOf  rdf:rest .

fc:Building  a           rdfs:Class , rdfs:Resource ;
        rdfs:comment     "The class of Buildings"@en ;
        rdfs:label       "Building"@en ;
        rdfs:subClassOf  rdfs:Resource , fc:Building .

rdf:List  a              rdfs:Class , rdfs:Resource ;
        rdfs:subClassOf  rdfs:Resource .

fc:studiesAt  a             rdf:Property , rdfs:Resource ;
        rdfs:comment        "Property describing that a living thing studies at a building or a location."@en ;
        rdfs:domain         fc:LivingBeings ;
        rdfs:label          "studies at"@en ;
        rdfs:range          fc:Building ;
        rdfs:subPropertyOf  fc:studiesAt .

fc:owns  a                  rdf:Property , rdfs:Resource ;
        rdfs:comment        "Property describing that a living thing owns a building or a location."@en ;
        rdfs:domain         fc:LivingBeings ;
        rdfs:label          "owns"@en ;
        rdfs:range          fc:Building ;
        rdfs:subPropertyOf  fc:owns .

rdf:predicate  a            rdf:Property , rdfs:Resource ;
        rdfs:domain         rdf:Statement ;
        rdfs:subPropertyOf  rdf:predicate .

rdf:Property  a          rdfs:Class , rdfs:Resource ;
        rdfs:subClassOf  rdfs:Resource , rdf:Property .

fc:Human  a              rdfs:Class , rdfs:Resource ;
        rdfs:comment     "The class of humans. Subclass of LivingBeings."@en ;
        rdfs:label       "Human"@en ;
        rdfs:subClassOf  rdfs:Resource , fc:LivingBeings , fc:Human .

rdfs:label  a       rdf:Property , rdfs:Resource ;
        rdfs:range  rdfs:Literal .

fc:Marriage  a           rdfs:Class , rdfs:Resource ;
        rdfs:subClassOf  rdfs:Resource , fc:Marriage .

fc:livesIn  a               rdf:Property , rdfs:Resource ;
        rdfs:comment        "Property describing that a living thing lives in a building or in a location."@en ;
        rdfs:domain         fc:LivingBeings ;
        rdfs:label          "lives in"@en ;
        rdfs:subPropertyOf  fc:livesIn .

rdf:Statement  a         rdfs:Class , rdfs:Resource ;
        rdfs:subClassOf  rdfs:Resource .

rdfs:Class  a            rdfs:Class , rdfs:Resource ;
        rdfs:subClassOf  rdfs:Resource , rdfs:Class .

rdf:type  a         rdf:Property , rdfs:Resource ;
        rdfs:range  rdfs:Class .

rdfs:Resource  a         rdfs:Class , rdfs:Resource ;
        rdfs:subClassOf  rdfs:Resource .

rdf:subject  a              rdf:Property , rdfs:Resource ;
        rdfs:domain         rdf:Statement ;
        rdfs:subPropertyOf  rdf:subject .

fc:Ownership  a          rdfs:Class , rdfs:Resource ;
        rdfs:subClassOf  rdfs:Resource , fc:Ownership .

rdf:XMLLiteral  a  rdfs:Datatype , rdfs:Class , rdfs:Resource .

rdfs:comment  a     rdf:Property , rdfs:Resource ;
        rdfs:range  rdfs:Literal .

fc:Animal  a             rdfs:Class , rdfs:Resource ;
        rdfs:comment     "The class of Animals. Subclass of LivingBeings"@en ;
        rdfs:label       "Animal"@en ;
        rdfs:subClassOf  rdfs:Resource , fc:LivingBeings , fc:Animal .

rdfs:range  a        rdf:Property , rdfs:Resource ;
        rdfs:domain  rdf:Property ;
        rdfs:range   rdfs:Class .

rdfs:subPropertyOf  a  rdf:Property , rdfs:Resource ;
        rdfs:domain  rdf:Property ;
        rdfs:range   rdf:Property .

rdf:object  a               rdf:Property , rdfs:Resource ;
        rdfs:domain         rdf:Statement ;
        rdfs:subPropertyOf  rdf:object .

fc:worksAt  a               rdf:Property , rdfs:Resource ;
        rdfs:comment        "Property describing that a living thing works at a building or at a location."@en ;
        rdfs:domain         fc:LivingBeings ;
        rdfs:label          "works at"@en ;
        rdfs:range          fc:Building ;
        rdfs:subPropertyOf  fc:worksAt .

fc:LivingBeings  a       rdfs:Class , rdfs:Resource ;
        rdfs:comment     "The class of living things."@en ;
        rdfs:label       "Living beings"@en ;
        rdfs:subClassOf  rdfs:Resource , fc:LivingBeings .

rdf:nil  a      rdf:List , rdfs:Resource .

rdfs:domain  a       rdf:Property , rdfs:Resource ;
        rdfs:domain  rdf:Property ;
        rdfs:range   rdfs:Class .

rdfs:Literal  a          rdfs:Class , rdfs:Resource ;
        rdfs:subClassOf  rdfs:Resource .

rdf:first  a                rdf:Property , rdfs:Resource ;
        rdfs:domain         rdf:List ;
        rdfs:subPropertyOf  rdf:first .

rdfs:subClassOf  a   rdf:Property , rdfs:Resource ;
        rdfs:domain  rdfs:Class ;
        rdfs:range   rdfs:Class .

fc:hasGender  a             rdf:Property , rdfs:Resource ;
        rdfs:comment        "Property describing that a living thing has a gender."@en ;
        rdfs:domain         fc:LivingBeings ;
        rdfs:label          "has gender"@en ;
        rdfs:range          fc:GenderType ;
        rdfs:subPropertyOf  fc:hasGender .

fc:GenderType  a         rdfs:Class , rdfs:Resource ;
        rdfs:comment     "The class of genders. "@en ;
        rdfs:label       "Gender type"@en ;
        rdfs:subClassOf  rdfs:Resource , fc:GenderType .

fc:Location  a           rdfs:Class , rdfs:Resource ;
        rdfs:comment     "The class of location"@en ;
        rdfs:label       "Location"@en ;
        rdfs:subClassOf  rdfs:Resource , fc:Location .

xsd:date  a              rdfs:Class , rdfs:Resource ;
        rdfs:subClassOf  rdfs:Resource , xsd:date .

fc:hasRelation  a           rdf:Property , rdfs:Resource ;
        rdfs:comment        "Property describing that a living thing has a relation with another living thing."@en ;
        rdfs:domain         fc:LivingBeings ;
        rdfs:range          fc:LivingBeings ;
        rdfs:subPropertyOf  fc:hasRelation .

fc:hasMarriageDate  a       rdf:Property , rdfs:Resource ;
        rdfs:comment        "Property describing that a living thing has a marriage date."@en ;
        rdfs:label          "has marriage date"@en ;
        rdfs:subPropertyOf  fc:hasEventDate , fc:hasMarriageDate .

fc:hasGrandMother  a        rdf:Property , rdfs:Resource ;
        rdfs:comment        "Property describing that a living thing has a grandmother. Subproperty of hasGrandMother."@en ;
        rdfs:label          "has grand mother"@en ;
        rdfs:subPropertyOf  fc:hasGrandParent , fc:hasGrandMother , fc:hasRelation , fc:hasAncestor , fc:hasBloodRelation .

fc:hasUncle  a              rdf:Property , rdfs:Resource ;
        rdfs:comment        "Property describing that a living thing has an uncle. Subproperty of hasBloodRelation."@en ;
        rdfs:label          "has uncle"@en ;
        rdfs:subPropertyOf  fc:hasBloodRelation , fc:hasUncle , fc:hasRelation .

fc:hasParent  a             rdf:Property , rdfs:Resource ;
        rdfs:comment        "Property describing that a living thing has a parent."@en ;
        rdfs:label          "has parent"@en ;
        rdfs:subPropertyOf  fc:hasAncestor , fc:hasParent , fc:hasRelation , fc:hasBloodRelation .

fc:hasSister  a             rdf:Property , rdfs:Resource ;
        rdfs:comment        "Property describing that a living thing has an a brother. Property describing that a living thing has an sister. Subproperty of hasSibling."@en ;
        rdfs:label          "has sister"@en ;
        rdfs:subPropertyOf  fc:hasSibling , fc:hasSister , fc:hasRelation , fc:hasBloodRelation .

fcsmps:Marge  a     fc:Woman , rdfs:Resource , fc:Human , fc:LivingBeings ;
        rdfs:label  "Marge Simpson" .

fc:hasGrandParent  a        rdf:Property , rdfs:Resource ;
        rdfs:comment        "Property describing that a living thing has a grandparent."@en ;
        rdfs:label          "has grand parent"@en ;
        rdfs:subPropertyOf  fc:hasAncestor , fc:hasGrandParent , fc:hasRelation , fc:hasBloodRelation .

fc:hasMother  a             rdf:Property , rdfs:Resource ;
        rdfs:comment        "Property describing that a living thing has a mother. Subproperty of hasParent."@en ;
        rdfs:label          "has mother"@en ;
        rdfs:subPropertyOf  fc:hasParent , fc:hasMother , fc:hasRelation , fc:hasAncestor , fc:hasBloodRelation .

fc:Woman  a              rdfs:Class , rdfs:Resource ;
        rdfs:comment     "The class of female humans. Subclass of Human."@en ;
        rdfs:label       "Woman"@en ;
        rdfs:subClassOf  fc:Human , fc:Woman , rdfs:Resource , fc:LivingBeings .

fc:hasWife  a               rdf:Property , rdfs:Resource ;
        rdfs:comment        "Property describing that a living thing has a wife. Subproperty of hasSpouse."@en ;
        rdfs:label          "has wife"@en ;
        rdfs:subPropertyOf  fc:hasSpouse , fc:hasWife , fc:hasRelation .

fc:Maleness  a           rdfs:Class , rdfs:Resource ;
        rdfs:comment     "The class of the male gender. Subclass of GenderType."@en ;
        rdfs:label       "Maleness"@en ;
        rdfs:subClassOf  fc:GenderType , fc:Maleness , rdfs:Resource .

fc:hasEventDate  a          rdf:Property , rdfs:Resource ;
        rdfs:domain         fc:LivingBeings ;
        rdfs:range          xsd:date ;
        rdfs:subPropertyOf  fc:hasEventDate .

fc:hasAncestor  a           rdf:Property , rdfs:Resource ;
        rdfs:comment        "Property describing that a living thing has an ancestor."@en ;
        rdfs:label          "has ancestor"@en ;
        rdfs:subPropertyOf  fc:hasBloodRelation , fc:hasAncestor , fc:hasRelation .

fc:hasSisterInLaw  a        rdf:Property , rdfs:Resource ;
        rdfs:comment        "Property describing that a living thing has a sister in law. Subproperty of hasSiblingInLaw."@en ;
        rdfs:label          "has sister in law"@en ;
        rdfs:subPropertyOf  fc:hasSiblingInLaw , fc:hasSisterInLaw , fc:hasRelation , fc:hasInlaw .

fc:hasBirthDate  a          rdf:Property , rdfs:Resource ;
        rdfs:comment        "Property describing that a living thing has a birth date."@en ;
        rdfs:label          "has birth date"@en ;
        rdfs:subPropertyOf  fc:hasEventDate , fc:hasBirthDate .

fc:hasDeathDate  a          rdf:Property , rdfs:Resource ;
        rdfs:comment        "Property describing that a living thing has death date."@en ;
        rdfs:label          "has death date"@en ;
        rdfs:subPropertyOf  fc:hasEventDate , fc:hasDeathDate .

fc:hasHusband  a            rdf:Property , rdfs:Resource ;
        rdfs:comment        "Property describing that a living thing has a husband. Subproperty of hasSpouse."@en ;
        rdfs:label          "has husband"@en ;
        rdfs:subPropertyOf  fc:hasSpouse , fc:hasHusband , fc:hasRelation .

fc:Femaleness  a         rdfs:Class , rdfs:Resource ;
        rdfs:comment     "The class of the female gender. Subclass of GenderType."@en ;
        rdfs:label       "Femaleness"@en ;
        rdfs:subClassOf  fc:GenderType , fc:Femaleness , rdfs:Resource .

fc:hasSibling  a            rdf:Property , rdfs:Resource ;
        rdfs:comment        "Property describing that a living thing has a sibling. Subproperty of hasBloodRelation."@en ;
        rdfs:label          "has sibling"@en ;
        rdfs:subPropertyOf  fc:hasBloodRelation , fc:hasSibling , fc:hasRelation .

fc:hasMotherInLaw  a        rdf:Property , rdfs:Resource ;
        rdfs:comment        "Property describing that a living thing has a mother in law. Subproperty of hasParentInLaw."@en ;
        rdfs:label          "has mother in law"@en ;
        rdfs:subPropertyOf  fc:hasParentInLaw , fc:hasMotherInLaw , fc:hasRelation , fc:hasInlaw .

fc:hasDivorceDate  a        rdf:Property , rdfs:Resource ;
        rdfs:comment        "Property describing that a living thing has a divorce date."@en ;
        rdfs:label          "has divorce date"@en ;
        rdfs:subPropertyOf  fc:hasEventDate , fc:hasDivorceDate .

fc:hasGrandFather  a        rdf:Property , rdfs:Resource ;
        rdfs:comment        "Property describing that a living thing has a grandfather. Subproperty of hasGrandParent."@en ;
        rdfs:label          "has grand father"@en ;
        rdfs:subPropertyOf  fc:hasGrandParent , fc:hasGrandFather , fc:hasRelation , fc:hasAncestor , fc:hasBloodRelation .

fc:hasBrother  a            rdf:Property , rdfs:Resource ;
        rdfs:comment        "Property describing that a living thing has an a brother. Property describing that a living thing has an aunt. Subproperty of hasSibling."@en ;
        rdfs:label          "has brother"@en ;
        rdfs:subPropertyOf  fc:hasSibling , fc:hasBrother , fc:hasRelation , fc:hasBloodRelation .

fc:hasSpouse  a             rdf:Property , rdfs:Resource ;
        rdfs:comment        "Property describing that a living thing has a spouse. Subproperty of hasRelation."@en ;
        rdfs:label          "has spouse"@en ;
        rdfs:subPropertyOf  fc:hasRelation , fc:hasSpouse .

fc:hasBloodRelation  a      rdf:Property , rdfs:Resource ;
        rdfs:comment        "Property describing that a living thing has a blood relation."@en ;
        rdfs:label          "has blood relation"@en ;
        rdfs:subPropertyOf  fc:hasRelation , fc:hasBloodRelation .

fc:hasInlaw  a              rdf:Property , rdfs:Resource ;
        rdfs:comment        "Property describing that a living thing has an in law."@en ;
        rdfs:label          "has inlaw"@en ;
        rdfs:subPropertyOf  fc:hasRelation , fc:hasInlaw .

fc:Man  a                rdfs:Class , rdfs:Resource ;
        rdfs:comment     "The class of male humans. Subclass of Human"@en ;
        rdfs:label       "Man"@en ;
        rdfs:subClassOf  fc:Human , fc:Man , rdfs:Resource , fc:LivingBeings .

fc:hasFatherInLaw  a        rdf:Property , rdfs:Resource ;
        rdfs:comment        "Property describing that a living thing has a father in law. Subproperty of hasParentInLaw."@en ;
        rdfs:label          "has father in law"@en ;
        rdfs:subPropertyOf  fc:hasParentInLaw , fc:hasFatherInLaw , fc:hasRelation , fc:hasInlaw .

fc:hasFather  a             rdf:Property , rdfs:Resource ;
        rdfs:comment        "Property describing that a living thing has a father. Subproperty of hasParent."@en ;
        rdfs:label          "has father"@en ;
        rdfs:subPropertyOf  fc:hasParent , fc:hasFather , fc:hasRelation , fc:hasAncestor , fc:hasBloodRelation .

fc:hasAunt  a               rdf:Property , rdfs:Resource ;
        rdfs:comment        "Property describing that a living thing has an aunt. Subproperty of hasBloodRelation."@en ;
        rdfs:label          "has aunt"@en ;
        rdfs:subPropertyOf  fc:hasBloodRelation , fc:hasAunt , fc:hasRelation .

fc:hasParentInLaw  a        rdf:Property , rdfs:Resource ;
        rdfs:comment        "Property describing that a living thing has a parent in law. Subproperty of hasInLaw."@en ;
        rdfs:label          "has parent in law"@en ;
        rdfs:subPropertyOf  fc:hasInlaw , fc:hasParentInLaw , fc:hasRelation .

fc:hasSiblingInLaw  a       rdf:Property , rdfs:Resource ;
        rdfs:comment        "Property describing that a living thing has a sibling in law. Subproperty of hasInLaw."@en ;
        rdfs:label          "has sibling in law"@en ;
        rdfs:subPropertyOf  fc:hasInlaw , fc:hasSiblingInLaw , fc:hasRelation .

fc:hasPet  a                rdf:Property , rdfs:Resource ;
        rdfs:comment        "Property describing that a living thing has a pet."@en ;
        rdfs:domain         fc:Human ;
        rdfs:label          "has pet"@en ;
        rdfs:range          fc:Animal ;
        rdfs:subPropertyOf  fc:hasRelation , fc:hasPet .

fc:hasBrotherInLaw  a       rdf:Property , rdfs:Resource ;
        rdfs:comment        "Property describing that a living thing has a brother in law. Subproperty of hasSiblingInLaw."@en ;
        rdfs:label          "has brother in law"@en ;
        rdfs:subPropertyOf  fc:hasSiblingInLaw , fc:hasBrotherInLaw , fc:hasRelation , fc:hasInlaw .

rdfs:Container  a        rdfs:Class , rdfs:Resource ;
        rdfs:subClassOf  rdfs:Container .

rdfs:ContainerMembershipProperty
        a                rdfs:Class , rdfs:Resource ;
        rdfs:subClassOf  rdfs:ContainerMembershipProperty , rdf:Property .

rdf:Bag  a               rdfs:Class , rdfs:Resource ;
        rdfs:subClassOf  rdf:Bag , rdfs:Container .

rdf:Seq  a               rdfs:Class , rdfs:Resource ;
        rdfs:subClassOf  rdf:Seq , rdfs:Container .

rdfs:Datatype  a         rdfs:Class , rdfs:Resource ;
        rdfs:subClassOf  rdfs:Datatype , rdfs:Class .

rdf:Alt  a               rdfs:Class , rdfs:Resource ;
        rdfs:subClassOf  rdf:Alt , rdfs:Container .

rdfs:isDefinedBy  a         rdf:Property , rdfs:Resource ;
        rdfs:subPropertyOf  rdfs:isDefinedBy , rdfs:seeAlso .

rdfs:seeAlso  a             rdf:Property , rdfs:Resource ;
        rdfs:subPropertyOf  rdfs:seeAlso .
