@prefix owl:   <http://www.w3.org/2002/07/owl#> .
@prefix rdf:   <http://www.w3.org/1999/02/22-rdf-syntax-ns#> .
@prefix xsd:   <http://www.w3.org/2001/XMLSchema#> .
@prefix rdfs:  <http://www.w3.org/2000/01/rdf-schema#> .
@prefix fcsmps: <http://example.org/fcsmps#> .
@prefix fc:    <http://example.org/fictionalchars#> .

fc:hasRelation  a     rdf:Property ;
        rdfs:comment  "Property describing that a living thing has a relation with another living thing."@en ;
        rdfs:domain   fc:LivingBeings ;
        rdfs:range    fc:LivingBeings .

fcsmps:Abraham  a      fc:Man ;
        rdfs:label     "Abraham Simpson" ;
        fc:hasBrother  fcsmps:Bill , fcsmps:Cyrus , fcsmps:Tyrone , fcsmps:Chet , fcsmps:Hubert ;
        fc:hasFather   fcsmps:Orville ;
        fc:hasGender   fc:Malesness ;
        fc:hasMother   fcsmps:Yuma ;
        fc:livesIn     fcsmps:Springfield .

fc:hasMarriageDate  a       rdf:Property ;
        rdfs:comment        "Property describing that a living thing has a marriage date."@en ;
        rdfs:label          "has marriage date"@en ;
        rdfs:subPropertyOf  fc:hasEventDate .

fcsmps:PowerPlant  rdfs:label  "Power Plant" ;
        rdfs:subClassOf  fc:Building .

fc:LivingBeings  a    rdfs:Class ;
        rdfs:comment  "The class of living things."@en ;
        rdfs:label    "Living beings"@en .

fcsmps:Snowball  a  fc:Animal ;
        rdfs:label  "Snowball II" ;
        fc:livesIn  fcsmps:Springfield .

fc:hasGrandMother  a        rdf:Property ;
        rdfs:comment        "Property describing that a living thing has a grandmother. Subproperty of hasGrandMother."@en ;
        rdfs:label          "has grand mother"@en ;
        rdfs:subPropertyOf  fc:hasGrandParent .

fc:hasUncle  a              rdf:Property ;
        rdfs:comment        "Property describing that a living thing has an uncle. Subproperty of hasBloodRelation."@en ;
        rdfs:label          "has uncle"@en ;
        rdfs:subPropertyOf  fc:hasBloodRelation .

fcsmps:SpringfieldPowerPlant
        a           fcsmps:PowerPlant ;
        rdfs:label  "Nuclear Power Plant" .

fc:Marriage  a  rdfs:Class .

fc:hasParent  a             rdf:Property ;
        rdfs:comment        "Property describing that a living thing has a parent."@en ;
        rdfs:label          "has parent"@en ;
        rdfs:subPropertyOf  fc:hasAncestor .

fcsmps:Jacqueline  a   fc:Woman ;
        rdfs:label     "Jacqueline Bouvier" ;
        fc:hasGender   fc:Femaleness ;
        fc:hasHusband  fcsmps:Clancy .

fc:hasSister  a             rdf:Property ;
        rdfs:comment        "Property describing that a living thing has an a brother. Property describing that a living thing has an sister. Subproperty of hasSibling."@en ;
        rdfs:label          "has sister"@en ;
        rdfs:subPropertyOf  fc:hasSibling .

fcsmps:Hubert  a       fc:Man ;
        rdfs:label     "Hubert Simpson" ;
        fc:hasBrother  fcsmps:Chet , fcsmps:Tyrone , fcsmps:Bill , fcsmps:Cyrus , fcsmps:Abraham ;
        fc:hasFather   fcsmps:Orville ;
        fc:hasGender   fc:Malesness ;
        fc:hasMother   fcsmps:Yuma .

fc:livesIn  a         rdf:Property ;
        rdfs:comment  "Property describing that a living thing lives in a building or in a location."@en ;
        rdfs:domain   fc:LivingBeings ;
        rdfs:label    "lives in"@en .

fcsmps:Marge  a        fc:Woman ;
        rdfs:label     "Marge Simpson" ;
        fc:hasFather   fcsmps:Clancy ;
        fc:hasGender   fc:Femaleness ;
        fc:hasHusband  fcsmps:Homer ;
        fc:hasMother   fcsmps:Jacqueline ;
        fc:hasSister   fcsmps:Selma , fcsmps:Patty ;
        fc:livesIn     fcsmps:Springfield .

fc:studiesAt  a       rdf:Property ;
        rdfs:comment  "Property describing that a living thing studies at a building or a location."@en ;
        rdfs:domain   fc:LivingBeings ;
        rdfs:label    "studies at"@en ;
        rdfs:range    fc:Building .

fc:hasGrandParent  a        rdf:Property ;
        rdfs:comment        "Property describing that a living thing has a grandparent."@en ;
        rdfs:label          "has grand parent"@en ;
        rdfs:subPropertyOf  fc:hasAncestor .

fc:hasMother  a             rdf:Property ;
        rdfs:comment        "Property describing that a living thing has a mother. Subproperty of hasParent."@en ;
        rdfs:label          "has mother"@en ;
        rdfs:subPropertyOf  fc:hasParent .

fc:Woman  a              rdfs:Class ;
        rdfs:comment     "The class of female humans. Subclass of Human."@en ;
        rdfs:label       "Woman"@en ;
        rdfs:subClassOf  fc:Human .

fc:hasWife  a               rdf:Property ;
        rdfs:comment        "Property describing that a living thing has a wife. Subproperty of hasSpouse."@en ;
        rdfs:label          "has wife"@en ;
        rdfs:subPropertyOf  fc:hasSpouse .

fc:owns  a            rdf:Property ;
        rdfs:comment  "Property describing that a living thing owns a building or a location."@en ;
        rdfs:domain   fc:LivingBeings ;
        rdfs:label    "owns"@en ;
        rdfs:range    fc:Building .

fc:Maleness  a           rdfs:Class ;
        rdfs:comment     "The class of the male gender. Subclass of GenderType."@en ;
        rdfs:label       "Maleness"@en ;
        rdfs:subClassOf  fc:GenderType .

fc:hasEventDate  a   rdf:Property ;
        rdfs:domain  fc:LivingBeings ;
        rdfs:range   xsd:date .

fc:hasAncestor  a           rdf:Property ;
        rdfs:comment        "Property describing that a living thing has an ancestor."@en ;
        rdfs:label          "has ancestor"@en ;
        rdfs:subPropertyOf  fc:hasBloodRelation .

fc:hasSisterInLaw  a        rdf:Property ;
        rdfs:comment        "Property describing that a living thing has a sister in law. Subproperty of hasSiblingInLaw."@en ;
        rdfs:label          "has sister in law"@en ;
        rdfs:subPropertyOf  fc:hasSiblingInLaw .

fc:hasBirthDate  a          rdf:Property ;
        rdfs:comment        "Property describing that a living thing has a birth date."@en ;
        rdfs:label          "has birth date"@en ;
        rdfs:subPropertyOf  fc:hasEventDate .

fc:Ownership  a  rdfs:Class .

fcsmps:Clancy  a      fc:Man ;
        rdfs:label    "Clancy Bouvier" ;
        fc:hasGender  fc:Malesness ;
        fc:hasWife    fcsmps:Jacqueline .

fc:Location  a        rdfs:Class ;
        rdfs:comment  "The class of location"@en ;
        rdfs:label    "Location"@en .

fc:hasDeathDate  a          rdf:Property ;
        rdfs:comment        "Property describing that a living thing has death date."@en ;
        rdfs:label          "has death date"@en ;
        rdfs:subPropertyOf  fc:hasEventDate .

fc:hasHusband  a            rdf:Property ;
        rdfs:comment        "Property describing that a living thing has a husband. Subproperty of hasSpouse."@en ;
        rdfs:label          "has husband"@en ;
        rdfs:subPropertyOf  fc:hasSpouse .

fc:Femaleness  a         rdfs:Class ;
        rdfs:comment     "The class of the female gender. Subclass of GenderType."@en ;
        rdfs:label       "Femaleness"@en ;
        rdfs:subClassOf  fc:GenderType .

fcsmps:Chet  a         fc:Man ;
        rdfs:label     "Chet Simpson" ;
        fc:hasBrother  fcsmps:Cyrus , fcsmps:Tyrone , fcsmps:Hubert , fcsmps:Abraham , fcsmps:Bill ;
        fc:hasFather   fcsmps:Orville ;
        fc:hasGender   fc:Malesness ;
        fc:hasMother   fcsmps:Yuma .

fc:GenderType  a      rdfs:Class ;
        rdfs:comment  "The class of genders. "@en ;
        rdfs:label    "Gender type"@en .

fc:hasSibling  a            rdf:Property ;
        rdfs:comment        "Property describing that a living thing has a sibling. Subproperty of hasBloodRelation."@en ;
        rdfs:label          "has sibling"@en ;
        rdfs:subPropertyOf  fc:hasBloodRelation .

fc:hasMotherInLaw  a        rdf:Property ;
        rdfs:comment        "Property describing that a living thing has a mother in law. Subproperty of hasParentInLaw."@en ;
        rdfs:label          "has mother in law"@en ;
        rdfs:subPropertyOf  fc:hasParentInLaw .

fc:hasDivorceDate  a        rdf:Property ;
        rdfs:comment        "Property describing that a living thing has a divorce date."@en ;
        rdfs:label          "has divorce date"@en ;
        rdfs:subPropertyOf  fc:hasEventDate .

fc:hasGender  a       rdf:Property ;
        rdfs:comment  "Property describing that a living thing has a gender."@en ;
        rdfs:domain   fc:LivingBeings ;
        rdfs:label    "has gender"@en ;
        rdfs:range    fc:GenderType .

fc:hasGrandFather  a        rdf:Property ;
        rdfs:comment        "Property describing that a living thing has a grandfather. Subproperty of hasGrandParent."@en ;
        rdfs:label          "has grand father"@en ;
        rdfs:subPropertyOf  fc:hasGrandParent .

fcsmps:Homer  a            fc:Man ;
        rdfs:label         "Homer Simpson" ;
        fc:hasFather       fcsmps:Abraham ;
        fc:hasGender       fc:Malesness ;
        fc:hasGrandFather  fcsmps:Orville ;
        fc:hasGrandMother  fcsmps:Yuma ;
        fc:hasMother       fcsmps:Mona ;
        fc:hasUncle        fcsmps:Bill , fcsmps:Tyrone , fcsmps:Chet , fcsmps:Cyrus , fcsmps:Hubert ;
        fc:hasWife         fcsmps:Marge ;
        fc:livesIn         fcsmps:Springfield ;
        fc:worksAt         fcsmps:SpringfieldPowerPlant .

fc:hasBrother  a            rdf:Property ;
        rdfs:comment        "Property describing that a living thing has an a brother. Property describing that a living thing has an aunt. Subproperty of hasSibling."@en ;
        rdfs:label          "has brother"@en ;
        rdfs:subPropertyOf  fc:hasSibling .

fc:worksAt  a         rdf:Property ;
        rdfs:comment  "Property describing that a living thing works at a building or at a location."@en ;
        rdfs:domain   fc:LivingBeings ;
        rdfs:label    "works at"@en ;
        rdfs:range    fc:Building .

fc:hasSpouse  a             rdf:Property ;
        rdfs:comment        "Property describing that a living thing has a spouse. Subproperty of hasRelation."@en ;
        rdfs:label          "has spouse"@en ;
        rdfs:subPropertyOf  fc:hasRelation .

fcsmps:Rita  a        fc:Woman ;
        rdfs:label    "Rita LaFleur Simpson" ;
        fc:hasGender  fc:Femaleness .

fc:hasBloodRelation  a      rdf:Property ;
        rdfs:comment        "Property describing that a living thing has a blood relation."@en ;
        rdfs:label          "has blood relation"@en ;
        rdfs:subPropertyOf  fc:hasRelation .

fcsmps:SantasHelper  a  fc:Animal ;
        rdfs:label  "Santas Little Helper" ;
        fc:livesIn  fcsmps:Springfield .

fc:hasInlaw  a              rdf:Property ;
        rdfs:comment        "Property describing that a living thing has an in law."@en ;
        rdfs:label          "has inlaw"@en ;
        rdfs:subPropertyOf  fc:hasRelation .

fcsmps:Mona  a         fc:Woman ;
        rdfs:label     "Mona Simpson" ;
        fc:hasGender   fc:Femaleness ;
        fc:hasHusband  fcsmps:Abraham .

fc:Human  a              rdfs:Class ;
        rdfs:comment     "The class of humans. Subclass of LivingBeings."@en ;
        rdfs:label       "Human"@en ;
        rdfs:subClassOf  fc:LivingBeings .

fc:Man  a                rdfs:Class ;
        rdfs:comment     "The class of male humans. Subclass of Human"@en ;
        rdfs:label       "Man"@en ;
        rdfs:subClassOf  fc:Human .

fc:hasFatherInLaw  a        rdf:Property ;
        rdfs:comment        "Property describing that a living thing has a father in law. Subproperty of hasParentInLaw."@en ;
        rdfs:label          "has father in law"@en ;
        rdfs:subPropertyOf  fc:hasParentInLaw .

fcsmps:Lisa  a             fc:Woman ;
        rdfs:label         "Lisa Simpson" ;
        fc:hasAunt         fcsmps:Patty , fcsmps:Selma ;
        fc:hasBrother      fcsmps:Bart ;
        fc:hasFather       fcsmps:Homer ;
        fc:hasGender       fc:Femaleness ;
        fc:hasGrandFather  fc:Abraham ;
        fc:hasGrandMother  fc:Mona ;
        fc:hasMother       fcsmps:Marge ;
        fc:hasPet          fcsmps:Snowball ;
        fc:hasSister       fcsmps:Maggie ;
        fc:hasUncle        fcsmps:Herbert ;
        fc:livesIn         fcsmps:Springfield .

fc:hasFather  a             rdf:Property ;
        rdfs:comment        "Property describing that a living thing has a father. Subproperty of hasParent."@en ;
        rdfs:label          "has father"@en ;
        rdfs:subPropertyOf  fc:hasParent .

fcsmps:Maggie  a           fc:Woman ;
        rdfs:label         "Maggie Simpson" ;
        fc:hasAunt         fcsmps:Patty , fcsmps:Selma ;
        fc:hasBrother      fcsmps:Bart ;
        fc:hasFather       fcsmps:Homer ;
        fc:hasGender       fc:Femaleness ;
        fc:hasGrandFather  fc:Abraham ;
        fc:hasGrandMother  fc:Mona ;
        fc:hasMother       fcsmps:Marge ;
        fc:hasSister       fcsmps:Lisa ;
        fc:hasUncle        fcsmps:Herbert ;
        fc:livesIn         fcsmps:Springfield .

fcsmps:Patty  a       fc:Woman ;
        rdfs:label    "Patty Bouvier" ;
        fc:hasFather  fcsmps:Clancy ;
        fc:hasGender  fc:Femaleness ;
        fc:hasMother  fcsmps:Jacqueline ;
        fc:livesIn    fcsmps:Springfield .

fcsmps:SpringfieldElementary
        a           fcsmps:School ;
        rdfs:label  "Springfield Elementary School" .

fcsmps:School  rdfs:label  "School" ;
        rdfs:subClassOf  fc:Building .

fc:hasAunt  a               rdf:Property ;
        rdfs:comment        "Property describing that a living thing has an aunt. Subproperty of hasBloodRelation."@en ;
        rdfs:label          "has aunt"@en ;
        rdfs:subPropertyOf  fc:hasBloodRelation .

fcsmps:Tyrone  a       fc:Man ;
        rdfs:label     "Tyrone Simpson" ;
        fc:hasBrother  fcsmps:Cyrus , fcsmps:Bill , fcsmps:Hubert , fcsmps:Abraham , fcsmps:Chet ;
        fc:hasFather   fcsmps:Orville ;
        fc:hasGender   fc:Malesness ;
        fc:hasMother   fcsmps:Yuma .

fcsmps:Bill  a         fc:Man ;
        rdfs:label     "Bill Simpson" ;
        fc:hasBrother  fcsmps:Cyrus , fcsmps:Hubert , fcsmps:Tyrone , fcsmps:Chet , fcsmps:Abraham ;
        fc:hasFather   fcsmps:Orville ;
        fc:hasGender   fc:Malesness ;
        fc:hasMother   fcsmps:Yuma .

fcsmps:Yuma  a        fc:Woman ;
        rdfs:label    "Yuma Hickman" ;
        fc:hasGender  fc:Femaleness .

fcsmps:Springfield  a  fc:Location ;
        rdfs:label  "Springfield" .

fcsmps:Orville  a     fc:Man ;
        rdfs:label    "Orville Simpson" ;
        fc:hasGender  fc:Malesness .

fc:Building  a        rdfs:Class ;
        rdfs:comment  "The class of Buildings"@en ;
        rdfs:label    "Building"@en .

fc:hasParentInLaw  a        rdf:Property ;
        rdfs:comment        "Property describing that a living thing has a parent in law. Subproperty of hasInLaw."@en ;
        rdfs:label          "has parent in law"@en ;
        rdfs:subPropertyOf  fc:hasInlaw .

fcsmps:Herbert  a          fc:Man ;
        rdfs:label         "Herbert Powell" ;
        fc:hasGender       fc:Malesness ;
        fc:hasGrandFather  fcsmps:Orville ;
        fc:hasGrandMother  fcsmps:Yuma ;
        fc:hasMother       fcsmps:Rita ;
        fc:hasUncle        fcsmps:Cyrus , fcsmps:Bill , fcsmps:Tyrone , fcsmps:Chet , fcsmps:Hubert .

fc:hasSiblingInLaw  a       rdf:Property ;
        rdfs:comment        "Property describing that a living thing has a sibling in law. Subproperty of hasInLaw."@en ;
        rdfs:label          "has sibling in law"@en ;
        rdfs:subPropertyOf  fc:hasInlaw .

fc:hasPet  a                rdf:Property ;
        rdfs:comment        "Property describing that a living thing has a pet."@en ;
        rdfs:domain         fc:Human ;
        rdfs:label          "has pet"@en ;
        rdfs:range          fc:Animal ;
        rdfs:subPropertyOf  fc:hasRelation .

fc:hasBrotherInLaw  a       rdf:Property ;
        rdfs:comment        "Property describing that a living thing has a brother in law. Subproperty of hasSiblingInLaw."@en ;
        rdfs:label          "has brother in law"@en ;
        rdfs:subPropertyOf  fc:hasSiblingInLaw .

fcsmps:Selma  a       fc:Woman ;
        rdfs:label    "Selma Bouvier" ;
        fc:hasFather  fcsmps:Clancy ;
        fc:hasGender  fc:Femaleness ;
        fc:hasMother  fcsmps:Jacqueline ;
        fc:livesIn    fcsmps:Springfield .

fc:Animal  a             rdfs:Class ;
        rdfs:comment     "The class of Animals. Subclass of LivingBeings"@en ;
        rdfs:label       "Animal"@en ;
        rdfs:subClassOf  fc:LivingBeings .

fcsmps:Bart  a             fc:Man ;
        rdfs:label         "Bart Simpson" ;
        fc:hasAunt         fcsmps:Selma , fcsmps:Patty ;
        fc:hasFather       fcsmps:Homer ;
        fc:hasGender       fc:Malesness ;
        fc:hasGrandFather  fc:Abraham ;
        fc:hasGrandMother  fc:Mona ;
        fc:hasMother       fcsmps:Marge ;
        fc:hasPet          fcsmps:SantasHelper ;
        fc:hasSister       fcsmps:Maggie , fcsmps:Lisa ;
        fc:hasUncle        fcsmps:Herbert ;
        fc:livesIn         fcsmps:Springfield .

fcsmps:Cyrus  a        fc:Man ;
        rdfs:label     "Cyrus Simpson" ;
        fc:hasBrother  fcsmps:Abraham , fcsmps:Hubert , fcsmps:Bill , fcsmps:Tyrone , fcsmps:Chet ;
        fc:hasFather   fcsmps:Orville ;
        fc:hasGender   fc:Malesness ;
        fc:hasMother   fcsmps:Yuma .
